\begin{example}
	Check that $y = t^2\ln{t}$ ($t > 0$) and $y = t^2$  are solutions to the differential equation.
	\begin{equation*}
		t^2y'' - 3ty' + 4y = 0
	\end{equation*}
\end{example}
\noindent
We'll check $y= t^2\ln{t}$ ($t > 0$) first.
\begin{equation*}
	t^2\left(t^2\ln{t}\right)'' - 3t\left(t^2\ln{t}\right)' + 4\left(t^2\ln{t}\right) = 0 \text{, } t > 0
\end{equation*}
\begin{equation*}
	t^2\left(3 + 2\ln{t}\right) - 3t\left(t + 2t\ln{t}\right) + 4\left(t^2\ln{t}\right) = 0 \text{, } t > 0
\end{equation*}
\begin{equation*}
	3t^2 + 2t^2\ln{t} - 3t^2 - 6t^2\ln{t} + 4t^2\ln{t} = 0 \text{, } t > 0
\end{equation*}
\begin{equation*}
	0 = 0
\end{equation*}
So $y = t^2\ln{t}$ ($t > 0$) is a solution.\\
Now we'll check $y= t^2$.
\begin{equation*}
	t^2\left(t^2\right)'' - 3t\left(t^2\right)' + 4\left(t^2\right) = 0
\end{equation*}
\begin{equation*}
	t^2\left(2\right) - 3t\left(2t\right) + 4t^2 = 0
\end{equation*}
\begin{equation*}
	2t^2 - 6t^2 + 4t^2 = 0
\end{equation*}
\begin{equation*}
	0 = 0
\end{equation*}
So $y = t^2$ is also a solution.