\subsubsection{Method of Lagrange Multipliers}
\noindent
Given an objective function, $f(x,y)$ and a constraint equation $g(x,y) = k$, define $F(x,y,\lambda) = f(x,y) + \lambda(k-g(x,y))$.
The solution, $(x, y, \lambda)$, to $\nabla F = \vec{0}$ will be the solution to the constrained optimization problem.\\

\noindent
For example, let's maximize $f(x,y)=xy$ subject to $(x-1)^2 + (y-1)^2 = 1$.
\begin{equation*}
	F(x,y,\lambda) = xy + \lambda(1 - (x-1)^2 - (y-1)^2)	
\end{equation*}
\begin{equation*}
	\nabla F = \langle y + 2\lambda(x-1), x+2\lambda(y-1), 1 - (x-1)^2 - (y-1)^2 = 1 \rangle = \vec{0}
\end{equation*}
\begin{equation*}
	\begin{cases}
		y - 2\lambda(x-1) = 0 \\ 
		x - 2\lambda(y-1) = 0 \\ 
		1 - (x-1)^2 - (y-1)^2 = 0
	\end{cases}
	\implies \begin{cases}
		y = 2\lambda(x-1) \\ 
		x = 2\lambda(y-1) \\ 
		(x-1)^2 + (y-1)^2 = 1
	\end{cases}
\end{equation*}
\begin{equation*}
	y = 2\lambda(2\lambda(y-1) - 1) = 4\lambda^2 y - 4\lambda^2 - 2\lambda = \frac{2\lambda}{2\lambda+1}
\end{equation*}
\begin{equation*}
	x = 2\lambda\left(\frac{2\lambda}{2\lambda+1} - 1\right) = \frac{2\lambda}{2\lambda+1} \implies x = y	
\end{equation*}
\begin{equation*}
	2(x-1)^2 = 1 \implies x = y = 1 \pm \frac{1}{\sqrt{2}}	
\end{equation*}
\begin{equation*}
	\implies \text{ Max/Min of } \frac{3 \pm 2\sqrt{2}}{2}.
\end{equation*}