\begin{example}
	Find the partial fraction decomposition of $\frac{2x-1}{x^3-6x^2+11x-6}$
\end{example}
\begin{answer}
	\begin{equation*}
		x^3-6x^2+11x-6 = (x-1)(x-2)(x-3).
	\end{equation*}
	So,
	\begin{equation*}
		\frac{2x-1}{x^3-6x^2+11x-6} = \frac{A_1}{x-1}+\frac{A_2}{x-2}+\frac{A_3}{x-3}.
	\end{equation*}
	Multiplying each side by the denominator,
	\begin{equation*}
		2x-1 = A_1(x-2)(x-3)+A_2(x-1)(x-3)+A_3(x-1)(x-2).
	\end{equation*}
	At $x=1$,
	\begin{equation*}
		1 = A_1(1-2)(1-3) \implies A_1 = \frac{1}{2}.
	\end{equation*}
	At $x=2$,
	\begin{equation*}
		3 = A_2(2-1)(2-3) \implies A_2 = -3.
	\end{equation*}
	At $x=3$,
	\begin{equation*}
		5 = A_3(3-1)(3-2) \implies A_3 = \frac{5}{2}.
	\end{equation*}
	So,
	\begin{equation*}
		\frac{2x-1}{x^3-6x^2+11x-6} = \frac{1/2}{x-1} + \frac{-3}{x-2} + \frac{5/2}{x-3},
	\end{equation*}
	just as was shown in the previous example.
\end{answer}