\begin{example}
	Find the general solution to the following equation
	\begin{equation*}
		y^{\prime\prime} + y = \csc{x}
	\end{equation*}
	given that $y_h = C_1\cos{x} + C_2\sin{x}$.
\end{example}
\noindent
$y_h$ gives us our two fundamental solutions
\begin{equation*}
	\begin{cases}
		y_1 = \cos{x} \\
		y_2 = \sin{x}
	\end{cases}
\end{equation*}
So, our system of equations is
\begin{equation*}
	\begin{cases}
		A^\prime\cos{x} + B^\prime\sin{x} = 0 \\
		-A^\prime\sin{x} + B^\prime\cos{x} = \csc{x}
	\end{cases} \to \begin{cases}
		A^\prime\cos{x} + B^\prime\sin{x} = 0 \\
		-A^\prime\cos{x} + B^\prime\frac{\cos^{2}{x}}{\sin{x}} = \frac{\cos{x}}{\sin^{2}{x}}
	\end{cases}
\end{equation*}
So, 
\begin{equation*}
	B^\prime\frac{1}{\sin{x}} = \frac{\cos{x}}{\sin^{2}{x}} \implies B^\prime = \frac{\cos{x}}{\sin{x}} = \cot{x} \implies B = \ln{\abs{\sin{x}}} + C_2
\end{equation*}
and
\begin{equation*}
	A^\prime\cos{x} + \cos{x} = 0 \implies A^\prime = -1 \implies A = -x + C_1
\end{equation*}
So, our general solution is
\begin{equation*}
	y = \left(C_1 - x\right)\cos{x} + \left(\ln{\abs{\sin{x}}} + C_2\right)\sin{x} = C_1\cos{x} + C_2\sin{x} - x\cos{x} + \sin{x}\ln{\abs{\sin{x}}}
\end{equation*}
Note how $y_h$ and $y_p$ appear together.