\begin{example}
	Find the general solution to the equation
	\begin{equation*}
		x^3y^{\prime\prime\prime} + x^2y^{\prime\prime} - 2xy^\prime = x^3\sin{x} \text{, } x > 0
	\end{equation*}
	given that $\left\{x, x^{-1}, x^2\right\}$ is the set of fundamental solutions.
\end{example}
\noindent
First we divide by $x^3$ to get a leading coefficient of 1.
\begin{equation*}
	y^{\prime\prime\prime} + x^{-1}y^{\prime\prime} - 2x^{-2}y^\prime = \sin{x} \text{, } x > 0
\end{equation*}
Next we calculate the $W(x)$ and each $W_i(x)$ for the fundamental solution set.
\begin{equation*}
	W[x,x^{-1}, x^2](x) = \begin{vmatrix}
		x & x^{-1} & x^2 \\
		1 & -x^{-2} & 2x \\
		0 & 2x^{-3} & 2
	\end{vmatrix} = 6x^{-1}
\end{equation*}
\begin{equation*}
	W_1(x) = (-1)^{3-1}W[x^{-1}, x^2](x) = (-1)^{2}\begin{vmatrix}
		x^{-1} & x^2 \\
		-x^{-2} & 2x
	\end{vmatrix} = 3
\end{equation*}
\begin{equation*}
	W_2(x) = (-1)^{3-2}\begin{vmatrix}
		x & x^{2} \\
		1 & 2x
	\end{vmatrix} = -x^2
\end{equation*}
\begin{equation*}
	W_2(x) = (-1)^{3-2}\begin{vmatrix}
		x & x^{-1} \\
		1 & -x^{-2}
	\end{vmatrix} = -2x^{-1}
\end{equation*}
Now we can calculate $y$.
\begin{equation*}
	y(x) = x\int{\frac{(\sin{x})^3}{-6x^{-1}} \mathrm{d}x} + x^{-1}\int{\frac{(\sin{x})(-x^2)}{-6x^{-1}} \mathrm{d}x} + x^2\int{\frac{(\sin{x})(-2x^{-1})}{-6x^{-1}} \mathrm{d}x}
\end{equation*}
\begin{equation*}
	= x\int{\left(\frac{-1}{2}x\sin{x}\right)\mathrm{d}x} + x^{-1}\int{\left(\frac{1}{6}x^3\sin{x}\right)\mathrm{d}x} + x^2\int{\left(\frac{1}{3}\sin{x}\right)\mathrm{d}x}
\end{equation*}
\begin{equation*}
	= C_1x + c_2x^{-1} + C_3x^2 + \cos{x} - x^{-1}\sin{x}
\end{equation*}