\subsection{Quotient Rule}
\begin{lemma}
	Let $f$ and $g$ be differentiable functions where $g \neq 0$. Then
	\begin{equation}
		\left(\frac{f}{g}\right)^\prime = \frac{gf^\prime - fg^\prime}{g^2}.
	\end{equation}
\end{lemma}
\begin{proof}
	Using the definition of the derivative and limit properties,
	\begin{align*}
		\left(\frac{f}{g}\right)^\prime &= \lim_{h\to 0}{\frac{\frac{f(x+h)}{g(x+h)} - \frac{f(x)}{g(x)}}{h}} \\
		&= \lim_{h\to 0}{\frac{1}{h}\frac{f(x+h)g(x) - f(x)g(x+h)}{g(x+h)g(x)}} \\
		&= \lim_{h\to 0}{\frac{1}{h}\hspace{3pt}\frac{f(x+h)g(x) - f(x)g(x) + f(x)g(x) - f(x)g(x+h)}{g(x+h)g(x)}} \\
		&= \lim_{h \to 0}{\frac{1}{g(x+h)g(x)}\hspace{3pt}\frac{f(x+h)g(x)-f(x)g(x)+f(x)g(x)-f(x)g(x+h)}{h}} \\
		&= \lim_{h \to 0}{\frac{1}{g(x+h)g(x)}\left(\frac{f(x+h)g(x)-f(x)g(x)}{h}+\frac{f(x)g(x)-f(x)g(x+h)}{h}\right)} \\
		&= \lim_{h \to 0}{\frac{1}{g(x+h)g(x)}} \left(g(x)\lim_{h \to 0}{\frac{f(x+h)-f(x)}{h}} - f(x)\lim_{h\to 0}{\frac{g(x+h)-g(x)}{h}}\right) \\
		&= \frac{1}{g^2(x)}\left(g(x)f^\prime(x) - f(x)g^\prime(x)\right) \\
		&= \frac{gf^\prime - fg^\prime}{g^2}.
	\end{align*}
\end{proof}

\begin{example}
	Given that the derivative of $\sin{(x)}$ is $\cos{(x)}$, find the derivative of $\frac{\sin{(x)}}{x^2}$.
\end{example}
Applying the quotient and power rules,
\begin{equation*}
	f^\prime(x) = \frac{x^2\cos{(x) - 2x\sin{(x)}}}{x^4} = \frac{x\cos{(x)}-2\sin{(x)}}{x^3}.
\end{equation*}